VCVio.lean
@@ -59,6 +59,8 @@ import VCVio.CryptoFoundations.UAKE.MessageTransmissionProtocol.Defs
 import VCVio.CryptoFoundations.UAKE.MessageTransmissionProtocol.OfAsymmEncAlg
 import VCVio.CryptoFoundations.UAKE.MessageTransmissionProtocol.OfSignatureAlg
 import VCVio.CryptoFoundations.UAKE.MessageTransmissionProtocol.Transcript
+import VCVio.CryptoFoundations.UAKE.MessageTransmissionProtocol.iCCA
+import VCVio.CryptoFoundations.UAKE.MessageTransmissionProtocol.iCMA
 import VCVio.EvalDist.BitVec
 import VCVio.EvalDist.Bool
 import VCVio.EvalDist.Defs.AlternativeMonad
